DumbContracts/Specs/SimpleStorage/Invariants.lean
@@ -6,6 +6,7 @@
 -/
 
 import DumbContracts.Core
+import DumbContracts.Specs.Common
 
 namespace DumbContracts.Specs.SimpleStorage
 
@@ -32,10 +33,6 @@ def map_storage_unchanged (s s' : ContractState) : Prop :=
   s'.storageMap = s.storageMap
 
 -- Context preservation: operations don't change sender/address
-def context_preserved (s s' : ContractState) : Prop :=
-  s'.sender = s.sender ∧
-  s'.thisAddress = s.thisAddress ∧
-  s'.msgValue = s.msgValue ∧
-  s'.blockTimestamp = s.blockTimestamp
+abbrev context_preserved := Specs.sameContext
 
 end DumbContracts.Specs.SimpleStorage
